add experimental features - verify contracts with [exists]

Generated/MATCH_RA2AK.bpl
@@ -1,47 +1,39 @@
 /*
-rule EA2A { 
-from 
-	att : ER!ERAttribute, 
-	ent : ER!Entity 
-	(att.entity = ent)
-to t : REL!RELAttribute 
-	( name <- att.name, 
-	  isKey <- att.isKey, 
-	  relation <- ent ) 
-}
- */
+rule RA2AK { from att : ER!ERAttribute, rse : ER!RelshipEnd 
+	           ( att.entity = rse.entity and att.isKey = true )
+	to   t : REL!RELAttribute 
+	         ( name <- att.name, isKey <- att.isKey, relation <- rse.relship )}
+*/
 
-
-
-procedure EA2A_match();
+procedure RA2AK_match();
 requires (forall att: ref :: att!=null && read($srcHeap, att, alloc) && dtype(att) == ER$ERAttribute ==> 
-			(forall ent: ref :: ent!=null && read($srcHeap, ent, alloc) && dtype(ent) == ER$Entity ==> 
-				$srcHeap[att, ERAttribute.entity] == ent ==>
-				getTarsBySrcs(Seq#Build(Seq#Singleton(att),ent))==null || !read($tarHeap, getTarsBySrcs(Seq#Build(Seq#Singleton(att),ent)), alloc)));
+			(forall rse: ref :: rse!=null && read($srcHeap, rse, alloc) && dtype(rse) == ER$RelshipEnd ==> 
+				($srcHeap[att, ERAttribute.entity] == $srcHeap[rse, RelshipEnd.entity] && $srcHeap[att, ERAttribute.isKey]) ==>
+					getTarsBySrcs(Seq#Build(Seq#Singleton(att),rse))==null || !read($tarHeap, getTarsBySrcs(Seq#Build(Seq#Singleton(att),rse)), alloc)));
 modifies $tarHeap,$linkHeap;
 ensures (forall att: ref :: att!=null && read($srcHeap, att, alloc) && dtype(att) == ER$ERAttribute ==> 
-			 (forall ent: ref :: ent!=null && read($srcHeap, ent, alloc) && dtype(ent) == ER$Entity ==> 
-				$srcHeap[att, ERAttribute.entity] == ent ==>
-				getTarsBySrcs(Seq#Build(Seq#Singleton(att),ent))!=null && read($tarHeap, getTarsBySrcs(Seq#Build(Seq#Singleton(att),ent)), alloc)));
+			 (forall rse: ref :: rse!=null && read($srcHeap, rse, alloc) && dtype(rse) == ER$RelshipEnd ==> 
+				($srcHeap[att, ERAttribute.entity] == $srcHeap[rse, RelshipEnd.entity] && $srcHeap[att, ERAttribute.isKey]) ==>
+					getTarsBySrcs(Seq#Build(Seq#Singleton(att),rse))!=null && read($tarHeap, getTarsBySrcs(Seq#Build(Seq#Singleton(att),rse)), alloc)));
 ensures (forall<alpha> $o : ref, $f: Field alpha ::
-	($o == null || read($tarHeap, $o, $f) == read(old($tarHeap), $o, $f) || (dtype($o) == REL$RELAttribute && dtype(Seq#Index(getTarsBySrcs_inverse($o), 0)) == ER$ERAttribute && dtype(Seq#Index(getTarsBySrcs_inverse($o), 1)) == ER$Entity && $f==alloc)));
+	($o == null || read($tarHeap, $o, $f) == read(old($tarHeap), $o, $f) || (dtype($o) == REL$RELAttribute && dtype(Seq#Index(getTarsBySrcs_inverse($o), 0)) == ER$ERAttribute && dtype(Seq#Index(getTarsBySrcs_inverse($o), 1)) == ER$RelshipEnd && $f==alloc)));
 free ensures $HeapSucc(old($tarHeap), $tarHeap);
 free ensures $HeapSucc(old($linkHeap), $linkHeap);
 free ensures surj_tar_model($srcHeap, $tarHeap);
 
-implementation EA2A_match () returns ()
+implementation RA2AK_match () returns ()
 {
 var stk: Seq BoxType;
 var $i: int;
 var $j: int;
 var att: ref;	//slot: 1
-var ent: ref;	//slot: 2
+var rse: ref;	//slot: 2
 var self: ref;	//slot: 0
 var obj#4: Seq ref;
 var obj#11: Seq ref;
-var cond#19: bool;
-var obj#24: ref;
-var obj#40: ref;
+var cond#25: bool;
+var obj#30: ref;
+var obj#46: ref;
 
 stk := OpCode#Aux#InitStk();
 
@@ -62,18 +54,18 @@ while($i<Seq#Length(obj#4))
   );
   invariant (forall i: int:: 0<=i &&i <$i ==>			
 			Seq#Index(obj#4,i)!=null && read($srcHeap, Seq#Index(obj#4,i), alloc) && dtype(Seq#Index(obj#4,i)) == ER$ERAttribute ==>
-			(forall o: ref :: Seq#Contains(Fun#LIB#AllInstanceFrom(old($srcHeap),ER$Entity),o) ==>		
-			o!=null && read($srcHeap, o, alloc) && dtype(o) == ER$Entity	==>
-				$srcHeap[Seq#Index(obj#4,i), ERAttribute.entity] == o ==>
+			(forall o: ref :: Seq#Contains(Fun#LIB#AllInstanceFrom(old($srcHeap),ER$RelshipEnd),o) ==>		
+			o!=null && read($srcHeap, o, alloc) && dtype(o) == ER$RelshipEnd	==>
+				($srcHeap[Seq#Index(obj#4,i), ERAttribute.entity] == $srcHeap[o, RelshipEnd.entity] && $srcHeap[Seq#Index(obj#4,i), ERAttribute.isKey]) ==>
 					getTarsBySrcs(Seq#Build(Seq#Singleton(Seq#Index(obj#4,i)),o))!=null 
 					&& read($tarHeap, getTarsBySrcs(Seq#Build(Seq#Singleton(Seq#Index(obj#4,i)),o)), alloc)
 			));
   invariant (forall<alpha> $o : ref, $f: Field alpha ::
-	($o == null || read($tarHeap, $o, $f) == read(old($tarHeap), $o, $f) || (dtype($o) == REL$RELAttribute && dtype(Seq#Index(getTarsBySrcs_inverse($o), 0)) == ER$ERAttribute && dtype(Seq#Index(getTarsBySrcs_inverse($o), 1)) == ER$Entity && $f==alloc)));
+	($o == null || read($tarHeap, $o, $f) == read(old($tarHeap), $o, $f) || (dtype($o) == REL$RELAttribute && dtype(Seq#Index(getTarsBySrcs_inverse($o), 0)) == ER$ERAttribute && dtype(Seq#Index(getTarsBySrcs_inverse($o), 1)) == ER$RelshipEnd && $f==alloc)));
 { 
 	stk := Seq#Build(stk, $Box(Seq#Index(obj#4, $i)));
 	call stk, att := OpCode#Store(stk);
-	call stk := OpCode#Push(stk, _Entity);
+	call stk := OpCode#Push(stk, _RelshipEnd);
 	call stk := OpCode#Push(stk, _ER);
 	call stk := OpCode#Findme(stk);
 	call stk := OpCode#Push(stk, _IN);
@@ -86,46 +78,68 @@ while($i<Seq#Length(obj#4))
 	while($j<Seq#Length(obj#11))
 	  invariant $j<=Seq#Length(obj#11);
 	  invariant (forall j: int:: 0<=j &&j <$j ==>			
-		Seq#Index(obj#11,j)!=null && read($srcHeap, Seq#Index(obj#11,j), alloc) && dtype(Seq#Index(obj#11,j)) == ER$Entity		
+		Seq#Index(obj#11,j)!=null && read($srcHeap, Seq#Index(obj#11,j), alloc) && dtype(Seq#Index(obj#11,j)) == ER$RelshipEnd		
 	  );
 	  invariant (forall j: int:: 0<=j &&j <$j ==>			
-			Seq#Index(obj#11,j)!=null && read($srcHeap, Seq#Index(obj#11,j), alloc) && dtype(Seq#Index(obj#11,j)) == ER$Entity	==>
-				$srcHeap[Seq#Index(obj#4,$i), ERAttribute.entity] == Seq#Index(obj#11,j) ==>
-					getTarsBySrcs(Seq#Build(Seq#Singleton(Seq#Index(obj#4,$i)),Seq#Index(obj#11,j)))!=null 
-					&& read($tarHeap, getTarsBySrcs(Seq#Build(Seq#Singleton(Seq#Index(obj#4,$i)),Seq#Index(obj#11,j))), alloc)
+			Seq#Index(obj#11,j)!=null && read($srcHeap, Seq#Index(obj#11,j), alloc) && dtype(Seq#Index(obj#11,j)) == ER$RelshipEnd	==>
+				($srcHeap[Seq#Index(obj#4,$i), ERAttribute.entity] == $srcHeap[Seq#Index(obj#11,j), RelshipEnd.entity] && $srcHeap[Seq#Index(obj#4,$i), ERAttribute.isKey]) ==>
+					getTarsBySrcs(Seq#Build(Seq#Singleton(Seq#Index(obj#4,$i)),Seq#Index(obj#11,j)))!=null && read($tarHeap, getTarsBySrcs(Seq#Build(Seq#Singleton(Seq#Index(obj#4,$i)),Seq#Index(obj#11,j))), alloc)
 			);
 	  invariant (forall i: int:: 0<=i &&i <$i ==>			
 			Seq#Index(obj#4,i)!=null && read($srcHeap, Seq#Index(obj#4,i), alloc) && dtype(Seq#Index(obj#4,i)) == ER$ERAttribute ==>
-			(forall o: ref :: Seq#Contains(Fun#LIB#AllInstanceFrom(old($srcHeap),ER$Entity),o) ==>		
-			o!=null && read($srcHeap, o, alloc) && dtype(o) == ER$Entity	==>
-				$srcHeap[Seq#Index(obj#4,i), ERAttribute.entity] == o ==>
+			(forall o: ref :: Seq#Contains(Fun#LIB#AllInstanceFrom(old($srcHeap),ER$RelshipEnd),o) ==>		
+			o!=null && read($srcHeap, o, alloc) && dtype(o) == ER$RelshipEnd ==>
+				($srcHeap[Seq#Index(obj#4,i), ERAttribute.entity] == $srcHeap[o, RelshipEnd.entity] && $srcHeap[Seq#Index(obj#4,i), ERAttribute.isKey]) ==>
 					getTarsBySrcs(Seq#Build(Seq#Singleton(Seq#Index(obj#4,i)),o))!=null 
 					&& read($tarHeap, getTarsBySrcs(Seq#Build(Seq#Singleton(Seq#Index(obj#4,i)),o)), alloc)
 			));
 	  invariant (forall<alpha> $o : ref, $f: Field alpha ::
-	($o == null || read($tarHeap, $o, $f) == read(old($tarHeap), $o, $f) || (dtype($o) == REL$RELAttribute && dtype(Seq#Index(getTarsBySrcs_inverse($o), 0)) == ER$ERAttribute && dtype(Seq#Index(getTarsBySrcs_inverse($o), 1)) == ER$Entity && $f==alloc)));
+	($o == null || read($tarHeap, $o, $f) == read(old($tarHeap), $o, $f) || (dtype($o) == REL$RELAttribute && dtype(Seq#Index(getTarsBySrcs_inverse($o), 0)) == ER$ERAttribute && dtype(Seq#Index(getTarsBySrcs_inverse($o), 1)) == ER$RelshipEnd && $f==alloc)));
 	{ 
 		stk := Seq#Build(stk, $Box(Seq#Index(obj#11, $j)));
-		call stk, ent := OpCode#Store(stk);
-		call stk := OpCode#Load(stk, att);
-
+		call stk, rse := OpCode#Store(stk);
 		
+
+		/* filter starts */
+		
+		call stk := OpCode#Load(stk, att);
 		assert Seq#Length(stk) >= 1;
 		assert $Unbox(Seq#Index(stk, Seq#Length(stk)-1)) != null;
 		stk := Seq#Build(Seq#Take(stk, Seq#Length(stk)-1), $Box($srcHeap[$Unbox(Seq#Index(stk, Seq#Length(stk)-1)), FieldOfDecl(dtype($Unbox(Seq#Index(stk, Seq#Length(stk)-1))), _Field$entity): Field (ref)]));
 			
 		//assert $Unbox(top(stk)) == $srcHeap[att, ERAttribute.entity];
 		
-		call stk := OpCode#Load(stk, ent);
+		call stk := OpCode#Load(stk, rse);
+		assert Seq#Length(stk) >= 1;
+		assert $Unbox(Seq#Index(stk, Seq#Length(stk)-1)) != null;
+		stk := Seq#Build(Seq#Take(stk, Seq#Length(stk)-1), $Box($srcHeap[$Unbox(Seq#Index(stk, Seq#Length(stk)-1)), FieldOfDecl(dtype($Unbox(Seq#Index(stk, Seq#Length(stk)-1))), _Field$entity): Field (ref)]));
+			
+		//assert $Unbox(top(stk)) == $srcHeap[rse, RelshipEnd.entity];
+		
 		call stk := OCL#Object#Equal(stk, $Unbox(Seq#Index(stk,Seq#Length(stk)-2)): ref, $Unbox(Seq#Index(stk,Seq#Length(stk)-1)): ref);
+		
+		call stk := OpCode#Load(stk, att);
+		assert Seq#Length(stk) >= 1;
+		assert $Unbox(Seq#Index(stk, Seq#Length(stk)-1)) != null;
+		stk := Seq#Build(Seq#Take(stk, Seq#Length(stk)-1), $Box($srcHeap[$Unbox(Seq#Index(stk, Seq#Length(stk)-1)), FieldOfDecl(dtype($Unbox(Seq#Index(stk, Seq#Length(stk)-1))), _Field$isKey): Field (bool)]));
+		
+		call stk := OpCode#Pusht(stk);
+		call stk := OCL#Object#Equal(stk, $Unbox(Seq#Index(stk,Seq#Length(stk)-2)): ref, $Unbox(Seq#Index(stk,Seq#Length(stk)-1)): ref);
+		
+		call stk := OCL#Boolean#And(stk);
 		call stk := OCL#Boolean#Not(stk);
-		cond#19 := $Unbox(Seq#Index(stk, Seq#Length(stk)-1));
-		call stk := OpCode#Pop(stk);
-		goto label_20, label_44;
-		label_20:
-			assume !cond#19;
+			
 
-			//assert $srcHeap[att, ERAttribute.entity] == ent;
+		cond#25 := $Unbox(Seq#Index(stk, Seq#Length(stk)-1));
+		call stk := OpCode#Pop(stk);
+		
+		/* filter ends */
+		
+		goto label_26, label_50;
+		label_26:
+			assume !cond#25;
+
+			//assert $srcHeap[att, ERAttribute.relship] == rse;
 			
 			call stk := OpCode#GetASM(stk);
 			
@@ -138,14 +152,14 @@ while($i<Seq#Length(obj#4))
 			
 			// new
 			assert Seq#Length(stk) >= 2;
-			havoc obj#24;
-			assume obj#24 != null && !read($linkHeap, obj#24, alloc) && dtype(obj#24) == 
+			havoc obj#30;
+			assume obj#30 != null && !read($linkHeap, obj#30, alloc) && dtype(obj#30) == 
 			classifierTable[($Unbox(Seq#Index(stk, Seq#Length(stk)-1)): String), 
 							($Unbox(Seq#Index(stk, Seq#Length(stk)-2)): String)];
-			$linkHeap := update($linkHeap, obj#24, alloc, true);
+			$linkHeap := update($linkHeap, obj#30, alloc, true);
 			assume $IsGoodHeap($linkHeap);
 			assume $HeapSucc(old($linkHeap), $linkHeap);
-			stk := Seq#Build(Seq#Take(stk, Seq#Length(stk)-2), $Box(obj#24));
+			stk := Seq#Build(Seq#Take(stk, Seq#Length(stk)-2), $Box(obj#30));
 			
 			
 			call stk := OpCode#Dup(stk);
@@ -167,8 +181,8 @@ while($i<Seq#Length(obj#4))
 			 $Unbox(Seq#Index(stk, Seq#Length(stk)-1)));
 
 			call stk := OpCode#Dup(stk);
-			call stk := OpCode#Push(stk, _ent);
-			call stk := OpCode#Load(stk, ent);
+			call stk := OpCode#Push(stk, _rse);
+			call stk := OpCode#Load(stk, rse);
 			
 			call stk := NTransientLink#addSourceElement
 			(stk, 
@@ -183,15 +197,15 @@ while($i<Seq#Length(obj#4))
 
 			// new
 			assert Seq#Length(stk) >= 2;
-			havoc obj#40;
-			assume obj#40 != null && !read($tarHeap, obj#40, alloc) && dtype(obj#40) == 
+			havoc obj#46;
+			assume obj#46 != null && !read($tarHeap, obj#46, alloc) && dtype(obj#46) == 
 			classifierTable[($Unbox(Seq#Index(stk, Seq#Length(stk)-1)): String), 
 							($Unbox(Seq#Index(stk, Seq#Length(stk)-2)): String)];
-			$tarHeap := update($tarHeap, obj#40, alloc, true);
+			$tarHeap := update($tarHeap, obj#46, alloc, true);
 			assume $IsGoodHeap($tarHeap);
 			assume $HeapSucc(old($tarHeap), $tarHeap);
-			assume getTarsBySrcs(Seq#Build(Seq#Singleton(att),ent)) == obj#40;
-			stk := Seq#Build(Seq#Take(stk, Seq#Length(stk)-2), $Box(obj#40));
+			assume getTarsBySrcs(Seq#Build(Seq#Singleton(att),rse)) == obj#46;
+			stk := Seq#Build(Seq#Take(stk, Seq#Length(stk)-2), $Box(obj#46));
 			
 			
 			call stk := NTransientLink#addTargetElement
@@ -204,8 +218,8 @@ while($i<Seq#Length(obj#4))
 			call stk := OpCode#Pusht(stk);
 			stk := Seq#Take(stk, Seq#Length(stk)-3);
 			goto done;
-		label_44:
-			assume cond#19; 
+		label_50:
+			assume cond#25; 
 			goto done;
 			
 		done:
@@ -221,13 +235,11 @@ while($i<Seq#Length(obj#4))
 
 assert (forall p: ref :: Seq#Contains(Fun#LIB#AllInstanceFrom(old($srcHeap),ER$ERAttribute),p) ==>			
 			p!=null && read($srcHeap, p, alloc) && dtype(p) == ER$ERAttribute ==>
-			(forall o: ref :: Seq#Contains(Fun#LIB#AllInstanceFrom(old($srcHeap),ER$Entity),o) ==>		
-			o!=null && read($srcHeap, o, alloc) && dtype(o) == ER$Entity	==>
-				$srcHeap[p, ERAttribute.entity] == o ==>
+			(forall o: ref :: Seq#Contains(Fun#LIB#AllInstanceFrom(old($srcHeap),ER$RelshipEnd),o) ==>		
+			o!=null && read($srcHeap, o, alloc) && dtype(o) == ER$RelshipEnd	==>
+				($srcHeap[p, ERAttribute.entity] == $srcHeap[o, RelshipEnd.entity] && $srcHeap[p, ERAttribute.isKey]) ==>
 					getTarsBySrcs(Seq#Build(Seq#Singleton(p),o))!=null 
 					&& read($tarHeap, getTarsBySrcs(Seq#Build(Seq#Singleton(p),o)), alloc)
 			));
 
 }
-
-
