Generated/Apply_RA2AK.bpl
@@ -1,0 +1,243 @@
+/*
+rule RA2AK { from att : ER!ERAttribute, rse : ER!RelshipEnd 
+	           ( att.entity = rse.entity and att.isKey = true )
+	to   t : REL!RELAttribute 
+	         ( name <- att.name, isKey <- att.isKey, relation <- rse.relship )}
+
+*/
+
+function RA2AK_links(
+	$srcHeap:HeapType,
+	$linkHeap:HeapType,
+	$tarHeap:HeapType,
+	links: Seq ref):bool
+{
+(forall att,rse: ref :: 
+	att!=null && read($srcHeap, att, alloc) && dtype(att) == ER$ERAttribute 
+ && rse!=null && read($srcHeap, rse, alloc) && dtype(rse) == ER$RelshipEnd ==> 
+		read($srcHeap, att, ERAttribute.entity) == read($srcHeap,rse, RelshipEnd.entity) && read($srcHeap,att,ERAttribute.isKey) ==>
+			(exists l:ref :: l!=null &&
+				Seq#Contains(links,l) && Map#Elements(read($linkHeap, l, TransientLink#source))[_att] == att  && Map#Elements(read($linkHeap, l, TransientLink#source))[_rse] == rse ))
+&&
+(forall i: int:: 0<=i &&i <Seq#Length(links) ==>			
+			Map#Elements($linkHeap[Seq#Index(links,i), TransientLink#target])[_t] != null 
+		 && read($tarHeap, Map#Elements($linkHeap[Seq#Index(links,i), TransientLink#target])[_t], alloc)
+		 && getTarsBySrcs(Seq#Build(Seq#Singleton(Map#Elements($linkHeap[Seq#Index(links,i), TransientLink#source])[_att]), Map#Elements($linkHeap[Seq#Index(links,i), TransientLink#source])[_rse])) == Map#Elements($linkHeap[Seq#Index(links,i), TransientLink#target])[_t]
+		)
+}
+
+
+
+procedure RA2AK_applys(links: Seq ref)
+requires $IsGoodHeap($tarHeap);
+requires links == NTransientLinkSet#getLinksByRule($linkHeap, _RA2AK);
+requires RA2AK_links($srcHeap,$linkHeap,$tarHeap,links);
+requires surj_tar_model($srcHeap, $tarHeap);
+requires (forall att,rse: ref :: 
+	att!=null && read($srcHeap, att, alloc) && dtype(att) == ER$ERAttribute 
+ && rse!=null && read($srcHeap, rse, alloc) && dtype(rse) == ER$RelshipEnd ==> 
+		read($srcHeap, att, ERAttribute.entity) == read($srcHeap,rse, RelshipEnd.entity) && read($srcHeap,att,ERAttribute.isKey) ==>
+		read($tarHeap, getTarsBySrcs(Seq#Build(Seq#Singleton(att),rse)), alloc) 
+	 && getTarsBySrcs(Seq#Build(Seq#Singleton(att),rse)) != null 
+	 && dtype(getTarsBySrcs(Seq#Build(Seq#Singleton(att),rse))) == REL$Relation	); // troublesome
+modifies $tarHeap;
+ensures (forall att,rse: ref :: 
+	att!=null && read($srcHeap, att, alloc) && dtype(att) == ER$ERAttribute 
+ && rse!=null && read($srcHeap, rse, alloc) && dtype(rse) == ER$RelshipEnd ==> 
+		read($srcHeap, att, ERAttribute.entity) == read($srcHeap,rse, RelshipEnd.entity) && read($srcHeap,att,ERAttribute.isKey) ==>
+		read($tarHeap, getTarsBySrcs(Seq#Build(Seq#Singleton(att),rse)), RELAttribute.name) == read($srcHeap, att, ERAttribute.name));
+ensures (forall att,rse: ref :: 
+	att!=null && read($srcHeap, att, alloc) && dtype(att) == ER$ERAttribute 
+ && rse!=null && read($srcHeap, rse, alloc) && dtype(rse) == ER$RelshipEnd ==> 
+		read($srcHeap, att, ERAttribute.entity) == read($srcHeap,rse, RelshipEnd.entity) && read($srcHeap,att,ERAttribute.isKey) ==>
+		read($tarHeap, getTarsBySrcs(Seq#Build(Seq#Singleton(att),rse)), RELAttribute.isKey) == read($srcHeap, att, ERAttribute.isKey));
+ensures (forall att,rse: ref :: 
+	att!=null && read($srcHeap, att, alloc) && dtype(att) == ER$ERAttribute 
+ && rse!=null && read($srcHeap, rse, alloc) && dtype(rse) == ER$RelshipEnd ==> 
+		read($srcHeap, att, ERAttribute.entity) == read($srcHeap,rse, RelshipEnd.entity) && read($srcHeap,att,ERAttribute.isKey) ==>
+		read($tarHeap, getTarsBySrcs(Seq#Build(Seq#Singleton(att),rse)), RELAttribute.relation) == getTarsBySrcs(Seq#Singleton(read($srcHeap,rse,RelshipEnd.relship))));
+ensures (forall<alpha> $o: ref, $f: Field alpha :: 
+	$o != null && read(old($tarHeap), $o, alloc) ==>
+		(  dtype($o) == REL$RELAttribute 
+		&& dtype(Seq#Index(getTarsBySrcs_inverse($o), 0)) == ER$ERAttribute 
+		&& dtype(Seq#Index(getTarsBySrcs_inverse($o), 1)) == ER$RelshipEnd 
+		&& ($f == RELAttribute.name || $f == RELAttribute.isKey || $f == RELAttribute.relation)) 
+	 || (read($tarHeap, $o, $f) == read(old($tarHeap), $o, $f)));
+ensures $HeapSucc(old($tarHeap), $tarHeap);
+ensures surj_tar_model($srcHeap, $tarHeap);
+{
+
+	var $i : int;
+	var link : ref;
+
+	
+	$i:=0;
+
+		
+	
+	while($i < Seq#Length(links))
+		invariant $i <= Seq#Length(links);
+		invariant surj_tar_model($srcHeap, $tarHeap);
+		invariant (forall i: int:: 0<=i &&i <$i ==>			
+			read($tarHeap, getTarsBySrcs(Seq#Build(Seq#Singleton(Map#Elements($linkHeap[Seq#Index(links,i), TransientLink#source])[_att]), Map#Elements($linkHeap[Seq#Index(links,i), TransientLink#source])[_rse])), RELAttribute.name) == $srcHeap[Map#Elements($linkHeap[Seq#Index(links,i), TransientLink#source])[_att], ERAttribute.name]
+		);
+		invariant (forall i: int:: 0<=i &&i <$i ==>			
+			read($tarHeap, getTarsBySrcs(Seq#Build(Seq#Singleton(Map#Elements($linkHeap[Seq#Index(links,i), TransientLink#source])[_att]), Map#Elements($linkHeap[Seq#Index(links,i), TransientLink#source])[_rse])), RELAttribute.isKey) == $srcHeap[Map#Elements($linkHeap[Seq#Index(links,i), TransientLink#source])[_att], ERAttribute.isKey]
+		);
+		invariant (forall i: int:: 0<=i &&i <$i ==>			
+			read($tarHeap, getTarsBySrcs(Seq#Build(Seq#Singleton(Map#Elements($linkHeap[Seq#Index(links,i), TransientLink#source])[_att]), Map#Elements($linkHeap[Seq#Index(links,i), TransientLink#source])[_rse])), RELAttribute.relation) == getTarsBySrcs(Seq#Singleton(read($srcHeap,Map#Elements($linkHeap[Seq#Index(links,i), TransientLink#source])[_rse],RelshipEnd.relship))));
+		invariant (forall<alpha> $o: ref, $f: Field alpha :: 
+	$o != null && read(old($tarHeap), $o, alloc) ==>
+		(  dtype($o) == REL$RELAttribute 
+		&& dtype(Seq#Index(getTarsBySrcs_inverse($o), 0)) == ER$ERAttribute 
+		&& dtype(Seq#Index(getTarsBySrcs_inverse($o), 1)) == ER$RelshipEnd 
+		&& ($f == RELAttribute.name || $f == RELAttribute.isKey || $f == RELAttribute.relation)) 
+	 || (read($tarHeap, $o, $f) == read(old($tarHeap), $o, $f)));
+		
+	{
+		link := Seq#Index(links, $i);			
+		call RA2AK_apply(link);
+		$i := $i+1;
+	}
+	
+	assume $HeapSucc(old($tarHeap), $tarHeap);
+}
+
+procedure RA2AK_apply (in: ref) returns ()
+  free requires surj_tar_model($srcHeap, $tarHeap);
+  free requires $linkHeap[in, TransientLink#rule]==_RA2AK;  
+  free requires $linkHeap[in, alloc] == true;
+  free requires dtype(in) == Native$TransientLink;
+  free requires Map#Domain($linkHeap[in, TransientLink#source])[_att];
+  free requires Map#Domain($linkHeap[in, TransientLink#source])[_rse];
+  free requires Map#Domain($linkHeap[in, TransientLink#target])[_t];
+  free requires dtype(Map#Elements($linkHeap[in, TransientLink#source])[_att]) == ER$ERAttribute;
+  free requires Map#Elements($linkHeap[in, TransientLink#source])[_att] != null;
+  free requires dtype(Map#Elements($linkHeap[in, TransientLink#source])[_rse]) == ER$RelshipEnd;
+  free requires Map#Elements($linkHeap[in, TransientLink#source])[_rse] != null;
+  free requires dtype(Map#Elements($linkHeap[in, TransientLink#target])[_t]) == REL$RELAttribute;
+  free requires Map#Elements($linkHeap[in, TransientLink#target])[_t] != null;
+  free requires getTarsBySrcs(Seq#Build(Seq#Singleton(Map#Elements($linkHeap[in, TransientLink#source])[_att]), Map#Elements($linkHeap[in, TransientLink#source])[_rse])) == Map#Elements($linkHeap[in, TransientLink#target])[_t];
+  free requires read($srcHeap, Map#Elements($linkHeap[in, TransientLink#source])[_att], ERAttribute.entity) == 
+  read($srcHeap,Map#Elements($linkHeap[in, TransientLink#source])[_rse], RelshipEnd.entity);
+  free requires read($srcHeap, Map#Elements($linkHeap[in, TransientLink#source])[_att], ERAttribute.isKey);
+  modifies $tarHeap;
+  ensures read($tarHeap, getTarsBySrcs(Seq#Build(Seq#Singleton(Map#Elements($linkHeap[in, TransientLink#source])[_att]), Map#Elements($linkHeap[in, TransientLink#source])[_rse])), RELAttribute.name) == read($srcHeap,Map#Elements($linkHeap[in, TransientLink#source])[_att],ERAttribute.name);
+  ensures read($tarHeap, getTarsBySrcs(Seq#Build(Seq#Singleton(Map#Elements($linkHeap[in, TransientLink#source])[_att]), Map#Elements($linkHeap[in, TransientLink#source])[_rse])), RELAttribute.isKey) == read($srcHeap,Map#Elements($linkHeap[in, TransientLink#source])[_att],ERAttribute.isKey);
+  ensures read($tarHeap, getTarsBySrcs(Seq#Build(Seq#Singleton(Map#Elements($linkHeap[in, TransientLink#source])[_att]), Map#Elements($linkHeap[in, TransientLink#source])[_rse])), RELAttribute.relation) == getTarsBySrcs(Seq#Singleton(read($srcHeap,Map#Elements($linkHeap[in, TransientLink#source])[_rse],RelshipEnd.relship)));
+  ensures (forall<alpha> $o: ref, $f: Field alpha :: 
+	$o != null && read(old($tarHeap), $o, alloc) ==>
+		(  dtype($o) == REL$RELAttribute 
+		&& dtype(Seq#Index(getTarsBySrcs_inverse($o), 0)) == ER$ERAttribute 
+		&& dtype(Seq#Index(getTarsBySrcs_inverse($o), 1)) == ER$RelshipEnd 
+		&& ($f == RELAttribute.name || $f == RELAttribute.isKey || $f == RELAttribute.relation)) 
+	 || (read($tarHeap, $o, $f) == read(old($tarHeap), $o, $f)));
+  ensures (forall<alpha> $o: ref, $f: Field alpha :: 
+	$o != null && read(old($tarHeap), $o, alloc) && $o != getTarsBySrcs(Seq#Build(Seq#Singleton(Map#Elements($linkHeap[in, TransientLink#source])[_att]), Map#Elements($linkHeap[in, TransientLink#source])[_rse])) ==> 
+	(read($tarHeap, $o, $f) == read(old($tarHeap), $o, $f))
+  );
+  ensures $HeapSucc(old($tarHeap), $tarHeap);
+  ensures surj_tar_model($srcHeap, $tarHeap);
+{
+
+var stk: Seq BoxType;
+var $i: int;
+var t: ref;	//slot: 4
+var att: ref;	//slot: 2
+var rse: ref;	//slot: 3
+var self: ref;	//slot: 0
+var link: ref;	//slot: 1
+stk := OpCode#Aux#InitStk();
+link := in;
+
+call stk := OpCode#Load(stk, link);
+call stk := OpCode#Push(stk, _att);
+call stk := NTransientLink#getSourceElement(
+				stk,
+				$Unbox(Seq#Index(stk, Seq#Length(stk)-2)),
+				$Unbox(Seq#Index(stk, Seq#Length(stk)-1)));
+call stk, att := OpCode#Store(stk);
+call stk := OpCode#Load(stk, link);
+call stk := OpCode#Push(stk, _rse);
+call stk := NTransientLink#getSourceElement(
+				stk,
+				$Unbox(Seq#Index(stk, Seq#Length(stk)-2)),
+				$Unbox(Seq#Index(stk, Seq#Length(stk)-1)));
+call stk, rse := OpCode#Store(stk);
+call stk := OpCode#Load(stk, link);
+call stk := OpCode#Push(stk, _t);
+call stk := NTransientLink#getTargetElement(
+				stk,
+				$Unbox(Seq#Index(stk, Seq#Length(stk)-2)),
+				$Unbox(Seq#Index(stk, Seq#Length(stk)-1)));
+call stk, t := OpCode#Store(stk);
+call stk := OpCode#Load(stk, t);
+call stk := OpCode#Dup(stk);
+call stk := OpCode#GetASM(stk);
+call stk := OpCode#Load(stk, att);
+
+// get
+assert Seq#Length(stk) >= 1;
+assert $Unbox(Seq#Index(stk, Seq#Length(stk)-1)) != null;
+stk := Seq#Build(Seq#Take(stk, Seq#Length(stk)-1), $Box($srcHeap[$Unbox(Seq#Index(stk, Seq#Length(stk)-1)), FieldOfDecl(dtype($Unbox(Seq#Index(stk, Seq#Length(stk)-1))), _Field$name): Field (String)]));
+
+call stk := ASM#Resolve(stk, $srcHeap, $Unbox(Seq#Index(stk, Seq#Length(stk)-1)): String);
+
+// set
+assert Seq#Length(stk) >= 2;
+assert $Unbox(Seq#Index(stk, Seq#Length(stk)-2)) != null;
+$tarHeap := update($tarHeap, $Unbox(Seq#Index(stk, Seq#Length(stk)-2)), 
+				FieldOfDecl(dtype($Unbox(Seq#Index(stk, Seq#Length(stk)-2))), _Field$name): Field (String), 
+				$Unbox(Seq#Index(stk, Seq#Length(stk)-1)));
+assume $IsGoodHeap($tarHeap);
+stk := Seq#Take(stk, Seq#Length(stk)-2);
+
+call stk := OpCode#Dup(stk);
+call stk := OpCode#GetASM(stk);
+call stk := OpCode#Load(stk, att);
+
+// get
+assert Seq#Length(stk) >= 1;
+assert $Unbox(Seq#Index(stk, Seq#Length(stk)-1)) != null;
+stk := Seq#Build(Seq#Take(stk, Seq#Length(stk)-1), $Box($srcHeap[$Unbox(Seq#Index(stk, Seq#Length(stk)-1)), FieldOfDecl(dtype($Unbox(Seq#Index(stk, Seq#Length(stk)-1))), _Field$isKey): Field (bool)]));
+
+call stk := ASM#Resolve(stk, $srcHeap, $Unbox(Seq#Index(stk, Seq#Length(stk)-1)): bool);
+
+// set
+assert Seq#Length(stk) >= 2;
+assert $Unbox(Seq#Index(stk, Seq#Length(stk)-2)) != null;
+$tarHeap := update($tarHeap, $Unbox(Seq#Index(stk, Seq#Length(stk)-2)), 
+				FieldOfDecl(dtype($Unbox(Seq#Index(stk, Seq#Length(stk)-2))), _Field$isKey): Field (bool), 
+				$Unbox(Seq#Index(stk, Seq#Length(stk)-1)));
+assume $IsGoodHeap($tarHeap);
+stk := Seq#Take(stk, Seq#Length(stk)-2);
+
+call stk := OpCode#Dup(stk);
+call stk := OpCode#GetASM(stk);
+call stk := OpCode#Load(stk, rse);
+
+
+// get
+assert Seq#Length(stk) >= 1;
+assert $Unbox(Seq#Index(stk, Seq#Length(stk)-1)) != null;
+stk := Seq#Build(Seq#Take(stk, Seq#Length(stk)-1), $Box($srcHeap[$Unbox(Seq#Index(stk, Seq#Length(stk)-1)), FieldOfDecl(dtype($Unbox(Seq#Index(stk, Seq#Length(stk)-1))), _Field$relship): Field (ref)]));
+
+
+call stk := ASM#Resolve(stk, $srcHeap, $Unbox(Seq#Index(stk, Seq#Length(stk)-1)): ref);
+assume $Unbox(Seq#Index(stk, Seq#Length(stk)-1)): ref == getTarsBySrcs(
+Seq#Singleton(read($srcHeap,Map#Elements($linkHeap[in, TransientLink#source])[_rse],RelshipEnd.relship)));
+
+
+// set
+assert Seq#Length(stk) >= 2;
+assert $Unbox(Seq#Index(stk, Seq#Length(stk)-2)) != null;
+$tarHeap := update($tarHeap, $Unbox(Seq#Index(stk, Seq#Length(stk)-2)), 
+				FieldOfDecl(dtype($Unbox(Seq#Index(stk, Seq#Length(stk)-2))), _Field$relation): Field (ref), 
+				$Unbox(Seq#Index(stk, Seq#Length(stk)-1)));
+assume $IsGoodHeap($tarHeap);
+stk := Seq#Take(stk, Seq#Length(stk)-2);
+
+
+call stk := OpCode#Pop(stk);
+
+}
